

Hyp: Let  $P(n)$  be the assertion that  $\text{medBin}$  works for all inputs  $\text{right-left}+1=n$ .

Base case: when  $n=1$  then  $\text{left}=\text{right}=m$  and  $A[m]=0/1$ . In case  $A[m]=0$  then as the function works 0 is returned. If  $A[m]=1$  then as the function works 1 is returned.

Inductive step: We assume  $\text{medBin}$  works as long as  $\text{right-left}+1 \leq k$ . We must prove  $\text{right-left}+1 \leq k+1$ . There are 4 cases. Where  $A[\text{left}]=A[\text{right}]$ ,  $A[m]=1 \wedge A[m-1]=0$ ,  $A[m]=1$ , and  $A[m]=0$ .

Case 1: ~~When~~  $A[\text{left}]=A[\text{right}]$

When  $A[\text{left}]=A[\text{right}]$  there are two sub cases. First  $A[\text{left}]=A[\text{right}]=1$ . Here 1 is returned as there is an amount of 1's. Second where  $A[\text{left}]=A[\text{right}]=0$ . Here 0 is returned as there are no 1's.

Case 2:  $A[m]=1 \wedge A[m-1]=0$

As the function works this will return  $n-m+1$  as that is the amount of 1's.

Case 3:  $A[m]=1$

We know the array is sorted and  $A[m-1]=1$  so the first occurrence of 1 must be between  $A[\text{left}]$  and  $A[m-1]$ . If the recursive call works correctly so shall this call. So  $n = (m-1) - \text{left} + 1$  or  $n = (\frac{\text{left}+\text{right}}{2} - 1) - \text{left} + 1$ . When  $\text{left}+\text{right}$  is even  $n = \frac{\text{right}+\text{left}}{2} - \frac{2\text{left}-1}{2} + 1 = \frac{\text{right}-\text{left}}{2}$ . When  $\text{right}+\text{left}$  is odd  $n = \frac{\text{right}+\text{left}+1}{2} - \frac{2\text{left}-1}{2} + 1 = \frac{\text{right}-\text{left}+1}{2} \leq \frac{\text{right}-\text{left}}{2} \leq \text{right}-\text{left}+1$  then  $\frac{\text{right}-\text{left}}{2} \leq k$ . Then the recursive call is made on interval 0 to  $k$  and is correct by Hyp thus working on  $k+1$ .

Case 4:  $A[m]=0$

This is symmetrical to the previous case as such  $n = \text{right} - (m+1) + 1 = \text{right} - (\frac{\text{left}+\text{right}}{2} + 1) + 1$ . When  $\text{right}+\text{left}$  is even then  $n = \frac{\text{right}-\text{left}}{2} - 1 + 1 = \frac{\text{right}-\text{left}}{2}$ . When  $\text{right}+\text{left}$  is odd then  $n = \frac{\text{right}-\text{left}+1}{2} - 1 + 1 = \frac{\text{right}-\text{left}+1}{2} \leq \text{right}-\text{left}+1 \leq k$  and  $\frac{\text{right}-\text{left}}{2} \leq k$ . Then the recursive call is made on interval 0 to  $k$  and is correct by Hyp thus working on  $k+1$ .

$\therefore$  As the inductive step works in all cases we can see  $\text{medBin}$  works in all cases.